#### Determination of Galvanoeter Resistance by Half Deflection Method-
$$ I_t = I_s + I_g $$
$$ I_t = \frac{E}{R_s + \frac{S \cdot (G+R_g)}{S+G+R_g}} $$
$$ I_g = \frac{S}{S+G+R_g} I_t $$
$$ Two\ cases\ where\ R_g=0\ and\ R_g=R_0 $$
$$ For\ R_g=0,\ I_{0} = \frac{S}{S+G} I_{t0} $$
$$ For\ R_g=R_0,\ I_g = \frac{S}{S+G+R_0} I_{tr0} $$
$$ As\ I_g<I_0\ half\ deflection\ method\ requires\ \frac{I_0}{I_g} = 2 $$
$$ General\ case,\ I_{t0} \not = I_{tr0}\ yields - $$
$$ => \frac{S+G+R_0}{S+G} \cdot \frac{I_{t0}}{I_{tr0}} = 2 $$
$$ => \frac{S+G+R_0}{S+G} \cdot \frac{R_s + \frac{S \cdot (G+R_0)}{S+G+R_0}}{R_s + \frac{S \cdot G}{S+G}} = 2 $$
$$ => \frac{R_s \cdot (S+G+R_0)+ S \cdot (G+R_0)}{R_s \cdot (S+R_0)+ S \cdot R_0} = 2 $$
$$ => R_s \cdot (S+G+R_0)+ S \cdot (G+R_0) = 2 \cdot (R_s \cdot (S+G)+ S \cdot G) $$
$$ => R_s \cdot (S+G+R_0-2S-2G)= S \cdot (2G - G -R_0) $$
$$ Let,\ \beta = \frac{R_s}{S} $$
$$ => \beta \cdot (R_0 - G - S) = G - R_0 $$
$$ => (1 + \beta) \cdot G = (1+ \beta)R_0 - \beta S $$
$$ Therefore,\ G = R_0 - \frac{\beta}{\beta +1}S \ .\ .\ .\ (General\ Formula)$$
$$ Let\ \alpha = \frac{S}{R_s} = \frac{1}{\beta} $$
$$ =>\ G = R_0 - \frac{ \frac {1}{\alpha} }{1+ \frac{1}{\alpha} }S $$
$$ =>\ G = R_0 - \frac{1}{1+\alpha}S ... (General) $$
$$ =>\ G=R_0 - (1 - \alpha + \alpha^2 - \alpha^3 + ...) S $$
$$ S << R_s\ implies\ \alpha \ \rightarrow \ 0 $$
$$ Then\ 1\ degree\ approximation\ yields- $$
$$ => G = R_0 - (1-\alpha)S $$
$$ 0\ degree\ apprximation\ yields- $$
$$ G = R_0 - S $$